Improved the marshall-predicate. It works much better now.

Java/src/Logic/ProtocolLogic.v
@@ -99,28 +99,21 @@ Instance EmbedPSasnSasnOp : EmbedOp sasn psasn := _.
 Instance EmbedPSasnSasn   : Embed sasn psasn := _.
 
 Module IsMarshallable.
-  Require Import Heap Relations RelationPairs.
+  Require Import Heap Relations RelationPairs ZArith.
   Import Marshall.
   
   Program Definition isMarshallable (v : var) (P : psasn) : psasn :=
   	fun PM STs s => mk_asn (fun Pr k h =>
-    	forall h' Pr' k' (Hk: k' <= k) (HPr: Prog_wf_sub Pr Pr'), P PM STs s Pr' k' h' -> marshall (s v) h h'
+    	forall m h' Pr' k' (Hsh: subheap h h') (Hsp: Prog_wf_sub Pr Pr'), 
+    	marshall Pr' (s v) h' m -> P PM STs s Pr' k' m
   	) _ _ _.
   Next Obligation.
-    eapply H with (k' := k').
-    omega.
-    apply HPr.
-    solve_model H0.
+    eapply H0; try eassumption.
+    transitivity P'; assumption.
   Defined.
   Next Obligation.
-    eapply H0. 
-    apply Hk.
-    transitivity P'; eassumption.
-    solve_model H1.
-  Defined.
-  Next Obligation.
-    eapply marshall_from_smaller; [eassumption |].
-    eapply H0; eassumption.
+    eapply H0; [ | assumption | eassumption].
+    transitivity h'; eassumption.
   Defined.
 
   Local Transparent EmbedILFunDropOp.
@@ -137,65 +130,32 @@ Module IsMarshallable.
   Local Existing Instance SepAlg_prod.
   Local Existing Instance UUSepAlg_prod.
 
-  Lemma pointsto_isMarshallable (p : var) (ptr : ptr) (f : field) (v : val) :
-    forall PM STs (s:stack) Pr k h  
-    (Href: s p = (vptr ptr)) (Hpointsto: (pointsto (vptr ptr) f v) Pr k h), 
-    (isMarshallable p (embed (pointsto (vptr ptr) f v))) PM STs s Pr k h
+  Lemma pointsto_isMarshallable_aux (p : var) (pos : nat) (cls : class) (f : field) (v : val) :
+    forall PM STs (s:stack) (Pr:Prog_wf) k h fields
+         (Href : s p = (vptr (pos, cls)))
+      (Hfields : field_lookup Pr cls fields)
+     (Hisfield : SS.In f fields)
+    (Hpointsto : (pointsto (vptr (pos, cls)) f v) Pr k h), 
+    (isMarshallable p (embed (pointsto (vptr (pos, cls)) f v))) PM STs s Pr k h
     .
   Proof.
-    admit.
-    (*
-    intros. 
-    simpl in Hpointsto.
-    
     simpl. intros.
-    destruct Hpointsto as [Hnotnull Hpointsto].
-    destruct H as [H'notnull H'pointsto].
-    unfold subheap in H'pointsto.
-    destruct H'pointsto as [h'' H'pointsto].
+    split; [apply Hpointsto |].
+    induction H; [
+    	rewrite Vint in Href |
+    	rewrite Vbool in Href |
+    	rewrite Vptr in Href
+    ]; inversion Href; subst.
+    inversion H1; subst; clear H1 Href.
+    exists (remove ((pos, cls), f) (get_heap_ptr m)).
+    apply sa_mul_swapL; [apply sa_mulC; apply uusa_unit; apply empty_1 |].
+    (* Make Hisfield talk about field0 *)
+    assert (SS.Equal fields fields0) by (eapply field_lookup_function_sub; eassumption).
+    rewrite H0 in Hisfield; clear H0.
+    (* And then use Mhere, now that we have the field0 evidence *)
+    apply Mhere; assumption.
+  Qed.
     
-    assert (h' = heap_add_ptr (mkheap h'' (get_heap_arr h')) ptr f v). admit.
-    rewrite H.
-    constructor. apply Href.
-    unfold subheap in Hpointsto; destruct Hpointsto as [? Hpointsto].
-    eapply sa_mul_mapstoL in Hpointsto.
-    apply Hpointsto.
-    apply add_1. reflexivity.
-    
-      unfold subheap in H'pointsto.
-      destruct H'pointsto as [h'' H'pointsto].
-      exists (mkheap h'' (get_heap_arr h')).
-      
-      split. intro key. unfold heap_add_ptr, mkheap, get_heap_arr; simpl.
-      simpl in H'pointsto.
-      specialize (H'pointsto key).
-      remember (find key (get_heap_ptr h')).
-      simpl in Heqo; rewrite <- Heqo in H'pointsto.
-      destruct o; unfold get_heap_ptr in Heqo; rewrite <- Heqo.
-      destruct H'pointsto as [[H'pointsto _] | [H'pointsto _]].
-      destruct (eq_dec key (ptr, f)).
-      rewrite H in H'pointsto.
-      apply map_mapsto_add_eq in H'pointsto; rewrite H'pointsto.
-      rewrite add_eq_o; [| auto]. reflexivity.
-      apply add_neq_mapsto_iff in H'pointsto; [| symmetry; auto].
-      apply empty_mapsto_iff in H'mapsto. inversion H'mapsto.
-      
-      apply find_mapsto_iff in H'pointsto. rewrite H'mapsto. reflexivity.
-      apply add_1; auto.
-      rewrite add_neq_o; [| symmetry; auto].
-      unfold sa_mul in H'pointsto. simpl in H'pointsto.
-      eapply sa_mul_mapstoR in H'pointsto.
-      destruct H'pointsto as [[H'mapsto _] | [H'mapsto _] ].
-      
-      apply add_neq_mapsto_iff in H'mapsto. apply empty_mapsto_iff in H'mapsto. inversion H'mapsto.
-      symmetry; apply H.
-      
-      SearchAbout MapsTo empty.
-      
-      
-    apply marshall_ptr.*)
-      Admitted.
-
 End IsMarshallable.
 
 
