Java/src/Logic/ST.v
@@ -58,175 +58,54 @@ Fixpoint subst_ST (x : var) (v : val) (t : ST) : ST :=
 
 Module Marshall.
 
-	Inductive marshall (v : sval) (big : heap) : heap -> Prop :=
-	  | marshall_int  : forall (z : Z)
-	                   (Vint : v = vint z),
-	                   marshall v big heap_unit
-	  | marshall_bool : forall (b : bool)
-	                    (Vbool : v = vbool b),
-	                    marshall v big heap_unit
-	  | marshall_ptr  : forall (ref : ptr) (f : field) (v' : sval) (m : heap)
-	                    (Vptr : v = vptr ref)
-	                    (Mmaps : MapsTo (ref, f) v' (get_heap_ptr big))
-	                    (Mmarshalls : marshall v' big m),
-	                    marshall v big (heap_add_ptr m ref f v')
+
+	Inductive marshall (Pr : Prog_wf) (v : sval) (big : heap) : heap -> Prop :=
+	  | marshall_int  : forall (z : Z) (m : heap)
+	                       (Vint : v = vint z)
+	                   (Msubheap : subheap m big),
+	                   marshall Pr v big m
+	  | marshall_bool : forall (b : bool) (m : heap)
+	                       (Vbool : v = vbool b)
+	                    (Msubheap : subheap m big),
+	                    marshall Pr v big m
+	  | marshall_ptr  : forall (ref : ptr) (cls : class) (pos : nat) (m : heap) fields
+	                        (Vptr : v = vptr ref)
+	                      (Vclass : ref = (pos, cls))
+	                     (Vfields : field_lookup Pr cls fields)
+	                       (Mhere : forall (f : field) (v' : sval),
+	                                SS.In f fields ->
+	                                MapsTo (ref, f) v' (get_heap_ptr big) /\
+	                                MapsTo (ref, f) v' (get_heap_ptr m))
+	                      (Mchild : forall (f : field) (v' : sval),
+	                                SS.In f fields ->
+	                                MapsTo (ref, f) v' (get_heap_ptr big) ->
+	                                marshall Pr v' big m
+	                      ),
+	                     marshall Pr v big m.
+	   (*            
 	  | marshall_arr  : forall (ref : arrptr) (i : nat) (v' : sval) (m : heap)
 	                    (Varr : v = varr ref)
 	                    (Mmaps : MapsTo (ref, i) v' (get_heap_arr big))
 	                    (Mmarshalls : marshall v' big m),
 	                    marshall v big (heap_add_arr m ref i v')
-	.
-
-	Lemma marshall_subheap {h h' : heap} {v : sval}
-	    (Hmarshall : marshall v h h') :
-	    subheap h' h.
+	.*)
+	
+	Lemma marshall_from_smaller {Pr : Prog_wf} {a b m : heap} {v : sval}
+	    (Hsubheap : subheap a b) (Hmarshall : marshall Pr v a m) :
+	    marshall Pr v b m.
 	Proof.
-	  assert (sa_unit heap_unit).
-	    unfold heap_unit; split; simpl; intuition.
-
-	  induction Hmarshall.
-	  + unfold subheap. exists big.
-	    apply sa_mulC.
-	    apply uusa_unit; assumption.
-	  + unfold subheap. exists big.
-	    apply sa_mulC.
-	    apply uusa_unit; assumption.
-	  + unfold subheap in IHHmarshall; destruct IHHmarshall as [h'' IHHmarshall].
-	    unfold subheap; exists (mkheap (remove (ref, f) (get_heap_ptr h'')) (get_heap_arr h'')).
-	    unfold heap_add_ptr.
-	    apply split_heap; [ repeat rewrite remove_mkheap_ptr | repeat rewrite remove_mkheap_arr ].
-	    * apply sa_mul_swapL; [apply IHHmarshall | apply Mmaps].
-	    * apply IHHmarshall. 
-	  + unfold subheap in IHHmarshall; destruct IHHmarshall as [h'' IHHmarshall].
-	    unfold subheap; exists (mkheap (get_heap_ptr h'') (remove (ref, i) (get_heap_arr h''))).
-	    unfold heap_add_arr.
-	    apply split_heap; [ repeat rewrite remove_mkheap_ptr | repeat rewrite remove_mkheap_arr ].
-	    * apply IHHmarshall.
-	    * apply sa_mul_swapL; [apply IHHmarshall | apply Mmaps].
-	Qed.
-
-	Lemma marshall_into_unit {m b} {v : sval}
-	    (Hempty : m === heap_unit) (Hmarshall : marshall v b m) :
-	    forall h, marshall v h m.
-	Proof.
-	  intro h.
-	  inversion Hmarshall.
-	  + eapply marshall_int; apply Vint.
-	  + eapply marshall_bool; apply Vbool.
-	  + destruct m as [m_ptr m_arr].
-	    assert (m_ptr === heap_ptr_unit) as Hempty_ptr by (apply Hempty).
-	    assert (Empty m_ptr) by (rewrite Hempty_ptr; intuition).
-	    unfold heap_add_ptr in H; simpl in H; unfold mkheap in H.
-	    inversion H.
-	    assert (MapsTo (ref, f) v' m_ptr) by (rewrite <- H2; apply add_1; reflexivity).
-	    unfold Empty in H0; specialize (H0 (ref, f) v').
-	    exfalso; auto.
-	  + destruct m as [m_ptr m_arr].
-	    assert (m_arr === heap_arr_unit) as Hempty_arr by (apply Hempty).
-	    assert (Empty m_arr) by (rewrite Hempty_arr; intuition).
-	    unfold heap_add_arr in H; simpl in H; unfold mkheap in H.
-	    inversion H.
-	    assert (MapsTo (ref, i) v' m_arr) by (rewrite <- H3; apply add_1; reflexivity).
-	    unfold Empty in H0; specialize (H0 (ref, i) v').
-	    exfalso; auto.
-	Qed.
-
-	Lemma marshall_into_smaller {a b c m : heap} {v : sval}
-	    (Habc : sa_mul a b c) (Hmarshall : marshall v c m)
-	    (Hdisjoint: DisjointHeaps b m) :
-	    marshall v a m \/ m === heap_unit.
-	Proof.
-	  induction Hmarshall; try auto; left.
-	  + constructor; try assumption.
-	    * eapply sa_mul_mapstoR in Mmaps; [| apply Habc].
-	      destruct Mmaps as [Mmaps | Mmaps]; destruct Mmaps as [Mmaps Mnotin]; [apply Mmaps|].
-	      unfold DisjointHeaps in Hdisjoint; destruct Hdisjoint as [Hdisjoint _].
-	      unfold Disjoint in Hdisjoint; specialize (Hdisjoint (ref, f)).
-	      exfalso; apply Hdisjoint. split.
-	      - unfold In; exists v'. assumption.
-	      - simpl. apply add_in_iff; auto. 
-	    * assert (DisjointHeaps b m). {
-	        unfold DisjointHeaps in *. destruct Hdisjoint as [Hdisjoint_ptr Hdisjoint_arr].
-	        split; [| apply Hdisjoint_arr]. simpl in Hdisjoint_ptr.
-	        unfold Disjoint in *. intro k. specialize (Hdisjoint_ptr k).
-	        intro Hcounter; apply Hdisjoint_ptr.
-	        destruct Hcounter as [Hcounter_b Hcounter_h'].
-	        split; [apply Hcounter_b|].
-	        destruct (eq_dec k (ref, f)); apply add_in_iff; auto.
-	      }
-	      apply IHHmarshall in Habc; [| apply H].
-	      destruct Habc; auto.
-	      eapply marshall_into_unit; [apply H0 | apply Hmarshall].
-	  + constructor; try assumption.
-	    * eapply sa_mul_mapstoR in Mmaps; [| apply Habc].
-	      destruct Mmaps as [Mmaps | Mmaps]; destruct Mmaps as [Mmaps Mnotin]; [apply Mmaps|].
-	      unfold DisjointHeaps in Hdisjoint; destruct Hdisjoint as [_ Hdisjoint].
-	      unfold Disjoint in Hdisjoint; specialize (Hdisjoint (ref, i)).
-	      exfalso; apply Hdisjoint. split.
-	      - unfold In; exists v'. assumption.
-	      - simpl. apply add_in_iff; auto.
-	    * assert (DisjointHeaps b m). {
-	        unfold DisjointHeaps in *. destruct Hdisjoint as [Hdisjoint_ptr Hdisjoint_arr].
-	        split; [apply Hdisjoint_ptr |]. simpl in Hdisjoint_arr.
-	        unfold Disjoint in *. intro k. specialize (Hdisjoint_arr k).
-	        intro Hcounter; apply Hdisjoint_arr.
-	        destruct Hcounter as [Hcounter_b Hcounter_h'].
-	        split; [apply Hcounter_b|].
-	        destruct (eq_dec k (ref, i)); apply add_in_iff; auto.
-	      }
-	      apply IHHmarshall in Habc; [| apply H].
-	      destruct Habc; auto.
-	      eapply marshall_into_unit; [apply H0 | apply Hmarshall].
-	Qed.
-
-	Lemma marshall_from_smaller {a b m : heap} {v : sval}
-	    (Hsubheap : subheap a b) (Hmarshall : marshall v a m) :
-	    marshall v b m.
-	Proof.
-	  induction Hmarshall.
-	  * eapply marshall_int; apply Vint.
-	  * eapply marshall_bool; apply Vbool.
-	  * eapply marshall_ptr.
-	    + apply Vptr.
-	    + unfold subheap in Hsubheap; destruct Hsubheap as [h Hsubheap].
-	      eapply sa_mul_mapstoL in Mmaps as [Mmaps Mnotin]; [| apply Hsubheap].
-	      apply Mmaps.
-	    + apply IHHmarshall; apply Hsubheap.
-	  * eapply marshall_arr.
-	    + apply Varr.
-	    + unfold subheap in Hsubheap; destruct Hsubheap as [h Hsubheap].
-	      eapply sa_mul_mapstoL in Mmaps as [Mmaps Mnotin]; [| apply Hsubheap].
-	      apply Mmaps.
-	    + apply IHHmarshall; apply Hsubheap.
-	Qed.
-
-	Lemma marshall_fails_outside {a b c m : heap} {v : sval}
-	    (Habc : sa_mul a b c) (Hmarshall : marshall v c m)
-	    (Hdisjoint: ~ DisjointHeaps b m) :
-	    ~ marshall v a m \/ m === heap_unit.
-	Proof.
-	  destruct (heap_eq_dec m heap_unit) as [Heq | Hneq]; [right; assumption |].
-	  apply overlapping_exists in Hdisjoint.
-	  destruct Hdisjoint.
-	  * destruct H as [ref [f [Hinb Hinm]]].
-	    assert (sa_mul (get_heap_ptr a) (get_heap_ptr b) (get_heap_ptr c)) as Habc_ptr by (apply Habc).
-	    apply sa_mulC2 in Habc_ptr.
-	    eapply sa_mul_inL in Habc_ptr; [ |apply Hinb]; destruct Habc_ptr as [Hnotina _].
-	    left; intro Hcounter.
-	    apply marshall_subheap in Hcounter.
-	    unfold subheap in Hcounter; destruct Hcounter as [d Hcounter].
-	    apply Hnotina.
-	    eapply sa_mul_inL; [apply Hcounter | apply Hinm].
-	  * destruct H as [ref [i [Hinb Hinm]]].
-	    assert (sa_mul (get_heap_arr a) (get_heap_arr b) (get_heap_arr c)) as Habc_arr by (apply Habc).
-	    apply sa_mulC2 in Habc_arr.
-	    eapply sa_mul_inL in Habc_arr; [ |apply Hinb]; destruct Habc_arr as [Hnotina _].
-	    left; intro Hcounter.
-	    apply marshall_subheap in Hcounter.
-	    unfold subheap in Hcounter; destruct Hcounter as [d Hcounter].
-	    apply Hnotina.
-	    eapply sa_mul_inL; [apply Hcounter | apply Hinm].
-  Qed.
+	    induction Hmarshall.
+	    * eapply marshall_int; [eassumption | transitivity big; assumption].
+	    * eapply marshall_bool; [eassumption | transitivity big; assumption].
+	    * eapply marshall_ptr; try eassumption; intros f v' Hin; specialize (Mhere f v' Hin).
+	      + destruct Mhere as [Minput Mres].
+	        split; [| assumption].
+	        destruct Hsubheap as [? Hsubheap].
+	        eapply sa_mul_mapstoL; [apply Hsubheap | apply Minput].
+	      + intro Hinput.
+	        destruct Mhere as [Minput Mres].
+	        eapply H; eassumption.
+    Qed.
 
 End Marshall.
 
